theories/Languages/Semantics.v
@@ -134,3 +134,142 @@ Proof.
   all: rewrite !(Eqdep_dec.UIP_dec type_dec _ eq_refl); cbn; try intros [=f]; auto.
   exact (f_equal _ eq).
 Defined.
+
+Inductive value : type -> Set :=
+  | VConst : forall {ty}, const ty -> value ty
+  | VIfte  : forall {ty}, value TBool -> value ty -> value ty -> value ty
+  | Vnot   : value TInt -> value TInt
+  | Vneg   : value TInt -> value TInt
+  | Vand   : value TBool -> value TBool -> value TBool
+  | Vor    : value TBool -> value TBool -> value TBool
+  | Vxor   : value TBool -> value TBool -> value TBool
+  | Vplus  : value TInt -> value TInt -> value TInt
+  | Vminus : value TInt -> value TInt -> value TInt
+  | Vmult  : value TInt -> value TInt -> value TInt
+  | Vdiv   : value TInt -> value TInt -> value TInt
+  | Veq    : value TInt -> value TInt -> value TBool
+  | Vneq   : value TInt -> value TInt -> value TBool
+  | Vle    : value TInt -> value TInt -> value TBool
+  | Vlt    : value TInt -> value TInt -> value TBool
+  | Vge    : value TInt -> value TInt -> value TBool
+  | Vgt    : value TInt -> value TInt -> value TBool
+.
+
+Lemma value_inv {ty} (x: value ty) :
+  {c : const ty | x = VConst c} +
+  {eb : value TBool & {et : value ty & {ef : value ty | x = VIfte eb et ef}}} +
+  {e: value TInt | exists (eqt : TInt = ty), x = eq_rect _ value (Vnot e) _ eqt} +
+  {e: value TInt | exists (eqt : TInt = ty), x = eq_rect _ value (Vneg e) _ eqt} +
+  {e1: value TBool & {e2 : value TBool | exists (eqt : TBool = ty), x = eq_rect _ value (Vand e1 e2) _ eqt}} +
+  {e1: value TBool & {e2 : value TBool | exists (eqt : TBool = ty), x = eq_rect _ value (Vor e1 e2) _ eqt}} +
+  {e1: value TBool & {e2 : value TBool | exists (eqt : TBool = ty), x = eq_rect _ value (Vxor e1 e2) _ eqt}} +
+  {e1: value TInt & {e2 : value TInt | exists (eqt : TInt = ty), x = eq_rect _ value (Vplus e1 e2) _ eqt}} +
+  {e1: value TInt & {e2 : value TInt | exists (eqt : TInt = ty), x = eq_rect _ value (Vminus e1 e2) _ eqt}} +
+  {e1: value TInt & {e2 : value TInt | exists (eqt : TInt = ty), x = eq_rect _ value (Vmult e1 e2) _ eqt}} +
+  {e1: value TInt & {e2 : value TInt | exists (eqt : TInt = ty), x = eq_rect _ value (Vdiv e1 e2) _ eqt}} +
+  {e1: value TInt & {e2 : value TInt | exists (eqt : TBool = ty), x = eq_rect _ value (Veq e1 e2) _ eqt}} +
+  {e1: value TInt & {e2 : value TInt | exists (eqt : TBool = ty), x = eq_rect _ value (Vneq e1 e2) _ eqt}} +
+  {e1: value TInt & {e2 : value TInt | exists (eqt : TBool = ty), x = eq_rect _ value (Vle e1 e2) _ eqt}} +
+  {e1: value TInt & {e2 : value TInt | exists (eqt : TBool = ty), x = eq_rect _ value (Vlt e1 e2) _ eqt}} +
+  {e1: value TInt & {e2 : value TInt | exists (eqt : TBool = ty), x = eq_rect _ value (Vge e1 e2) _ eqt}} +
+  {e1: value TInt & {e2 : value TInt | exists (eqt : TBool = ty), x = eq_rect _ value (Vgt e1 e2) _ eqt}}.
+Proof using.
+  destruct x.
+  1-16: left.
+  1-15: left.
+  1-14: left.
+  1-13: left.
+  1-12: left.
+  1-11: left.
+  1-10: left.
+  1-9: left.
+  1-8: left.
+  1-7: left.
+  1-6: left.
+  1-5: left.
+  1-4: left.
+  1-3: left.
+  1-2: left.
+  1-1: left.
+  2-17: right.
+  all: repeat (eexists; try exists eq_refl).
+Defined.
+
+Lemma value_dec {ty} (v1 v2: value ty) : {v1 = v2} + {v1 <> v2}.
+Proof.
+  revert v2.
+  induction v1 as [ty1 c1 | ty1 vb1 IHeb1 vt1 IHvt1 vf1 IHvf1 | v1 IH | v1 IH | v11 IH1 v12 IH2 | v11 IH1 v12 IH2 | v11 IH1 v12 IH2 | v11 IH1 v12 IH2 | v11 IH1 v12 IH2 | v11 IH1 v12 IH2 | v11 IH1 v12 IH2 | v11 IH1 v12 IH2 | v11 IH1 v12 IH2 | v11 IH1 v12 IH2 | v11 IH1 v12 IH2 | v11 IH1 v12 IH2 | v11 IH1 v12 IH2].
+  all: intro v2.
+  1, 2: destruct (value_inv v2) as [[[[[[[[[[[[[[[[
+    (c2 & ->) | (vb2 & vt2 & vf2 & ->)] |
+    (v2' & eqt2)] |
+    (v2' & eqt2)] |
+    (v21 & v22 & eqt2)] |
+    (v21 & v22 & eqt2)] |
+    (v21 & v22 & eqt2)] |
+    (v21 & v22 & eqt2)] |
+    (v21 & v22 & eqt2)] |
+    (v21 & v22 & eqt2)] |
+    (v21 & v22 & eqt2)] |
+    (v21 & v22 & eqt2)] |
+    (v21 & v22 & eqt2)] |
+    (v21 & v22 & eqt2)] |
+    (v21 & v22 & eqt2)] |
+    (v21 & v22 & eqt2)] |
+    (v21 & v22 & eqt2)]; try (right; (try destruct eqt2); subst; simpl; discriminate).
+  1: destruct (const_dec c1 c2); [left; subst; reflexivity | right; intros [=f]; apply sig2T_eq_type in f; contradiction].
+  1: destruct (IHeb1 vb2).
+  2: right; intros [=f]; contradiction.
+  1: destruct (IHvt1 vt2).
+  2: right; intros [=_ f]; apply sig2T_eq_type in f; contradiction.
+  1: destruct (IHvf1 vf2).
+  2: right; intros [=_ _ f]; apply sig2T_eq_type in f; contradiction.
+  1: subst; left; reflexivity.
+  1, 2: destruct (value_inv v2) as [[[[[[[[[[[[[[[[
+    (c2 & ->) | (vb2 & vt2 & vf2 & ->)] |
+    (v2' & eqt2)] |
+    (v2' & eqt2)] |
+    (v21 & v22 & eqt2)] |
+    (v21 & v22 & eqt2)] |
+    (v21 & v22 & eqt2)] |
+    (v21 & v22 & eqt2)] |
+    (v21 & v22 & eqt2)] |
+    (v21 & v22 & eqt2)] |
+    (v21 & v22 & eqt2)] |
+    (v21 & v22 & eqt2)] |
+    (v21 & v22 & eqt2)] |
+    (v21 & v22 & eqt2)] |
+    (v21 & v22 & eqt2)] |
+    (v21 & v22 & eqt2)] |
+    (v21 & v22 & eqt2)]; try (right; (try destruct eqt2); subst; simpl; discriminate); try (right; destruct eqt2 as [type_eq eqt2]; revert eqt2; refine (match type_eq with eq_refl => fun f => _ end); subst; discriminate).
+    1, 2: destruct (IH v2') as [eq|neq]; [left | right].
+    1-4: destruct eqt2 as [type_eq ->].
+    1, 3: exact (match type_eq with eq_refl => f_equal _ eq end).
+    1, 2: refine (match type_eq with eq_refl => fun f => _ end); cbn in f.
+    1, 2: injection f as f; exact (neq f).
+  all: destruct (value_inv v2) as [[[[[[[[[[[[[[[[
+    (c2 & ->) | (vb2 & vt2 & vf2 & ->)] |
+    (v2' & eqt2)] |
+    (v2' & eqt2)] |
+    (v21 & v22 & eqt2)] |
+    (v21 & v22 & eqt2)] |
+    (v21 & v22 & eqt2)] |
+    (v21 & v22 & eqt2)] |
+    (v21 & v22 & eqt2)] |
+    (v21 & v22 & eqt2)] |
+    (v21 & v22 & eqt2)] |
+    (v21 & v22 & eqt2)] |
+    (v21 & v22 & eqt2)] |
+    (v21 & v22 & eqt2)] |
+    (v21 & v22 & eqt2)] |
+    (v21 & v22 & eqt2)] |
+    (v21 & v22 & eqt2)]; try (right; (try destruct eqt2); subst; simpl; discriminate); try (right; destruct eqt2 as [type_eq eqt2]; revert eqt2; refine (match type_eq with eq_refl => fun f => _ end); subst; discriminate).
+    all: destruct (IH1 v21) as [eq1|neq1]; [| right].
+    all: try (destruct (IH2 v22) as [eq2|neq2]; [left| right]).
+    all: subst.
+    all: destruct eqt2 as [type_eq ->].
+    all: try exact (match type_eq with eq_refl => eq_refl end).
+    all: refine (match type_eq with eq_refl => fun f => _ end); cbn in f.
+    all: injection f as f.
+    all: contradiction.
+Qed.
